theories/reactive/utp_rea_healths.thy
@@ -122,10 +122,10 @@ lemma R1_skip: "R1(II) = II"
 lemma skip_is_R1 [closure]: "II is R1"
   by (rel_auto)
 
-lemma subst_R1: "\<lbrakk> $tr \<sharp> \<sigma>; $tr\<acute> \<sharp> \<sigma>  \<rbrakk> \<Longrightarrow> \<sigma> \<dagger> (R1 P) = R1(\<sigma> \<dagger> P)"
+lemma subst_R1: "\<lbrakk> $tr \<sharp>\<^sub>s \<sigma>; $tr\<acute> \<sharp>\<^sub>s \<sigma>  \<rbrakk> \<Longrightarrow> \<sigma> \<dagger> (R1 P) = R1(\<sigma> \<dagger> P)"
   by (simp add: R1_def usubst)
   
-lemma subst_R1_closed [closure]: "\<lbrakk> $tr \<sharp> \<sigma>; $tr\<acute> \<sharp> \<sigma>; P is R1 \<rbrakk> \<Longrightarrow> \<sigma> \<dagger> P is R1"
+lemma subst_R1_closed [closure]: "\<lbrakk> $tr \<sharp>\<^sub>s \<sigma>; $tr\<acute> \<sharp>\<^sub>s \<sigma>; P is R1 \<rbrakk> \<Longrightarrow> \<sigma> \<dagger> P is R1"
   by (metis Healthy_def subst_R1)
 
 lemma R1_by_refinement:
